execution/tests/DexterTests/DexterTests.v
@@ -104,13 +104,13 @@ Definition chain0 : ChainBuilder :=
 Definition chain1 : ChainBuilder :=
   unpack_result (TraceGens.add_block chain0
   [
-    build_act creator (act_transfer person_1 10) ;
-    build_act creator deploy_fa2token ;
-    build_act creator deploy_dexter ;
-    build_act creator deploy_exploit ;
-    build_act person_1 (act_call fa2_caddr 10%Z (serialize _ _ (msg_create_tokens 0%N))) ;
-    build_act creator (act_call dexter_caddr 10%Z (serialize _ _ (dexter_other_msg (add_to_tokens_reserve 0%N)))) ;
-    build_act person_1 (act_call fa2_caddr 0%Z  (serialize _ _ (msg_update_operators [add_operator (add_operator_all person_1 exploit_caddr);
+    build_act creator creator (act_transfer person_1 10) ;
+    build_act creator creator deploy_fa2token ;
+    build_act creator creator deploy_dexter ;
+    build_act creator creator deploy_exploit ;
+    build_act person_1 person_1 (act_call fa2_caddr 10%Z (serialize _ _ (msg_create_tokens 0%N))) ;
+    build_act creator creator (act_call dexter_caddr 10%Z (serialize _ _ (dexter_other_msg (add_to_tokens_reserve 0%N)))) ;
+    build_act person_1 person_1 (act_call fa2_caddr 0%Z  (serialize _ _ (msg_update_operators [add_operator (add_operator_all person_1 exploit_caddr);
                                                                                       add_operator (add_operator_all person_1 dexter_caddr)])))
   ]).
 
@@ -137,12 +137,11 @@ Definition call_dexter owner_addr :=
     transfer_descr_batch := [];
     transfer_descr_operator := dexter_caddr;
   |} in
-  build_act owner_addr (act_call exploit_caddr 0%Z (@serialize _ _ (tokens_sent dummy_descriptor))).
+  build_act owner_addr owner_addr (act_call exploit_caddr 0%Z (@serialize _ _ (tokens_sent dummy_descriptor))).
 
 Definition gExploitAction : GOpt Action :=
-  bindGen (elems [person_1; person_2; person_3]) (fun addr =>
-    returnGenSome (call_dexter addr)
-  ).
+  bindGen (elems [person_1; person_2; person_3])
+          (fun addr => returnGenSome (call_dexter addr)).
 
 Definition gExploitChainTraceList max_acts_per_block cb length :=
   gChain cb (fun cb _ => gExploitAction) length 1 max_acts_per_block.
@@ -202,7 +201,6 @@ Definition tokens_to_asset_correct_P env :=
 
 Definition tokens_to_asset_correct :=
   forAllBlocks 1 chain1 (gExploitChainTraceList 1) tokens_to_asset_correct_P.
-(* QuickChick tokens_to_asset_correct. *)
 
 (* Illustration of how the reentrancy attack can give the caller more money with the same amount of tokens.
    Notice how in the second sequence, the second argument remains the same, ie. it emulates the reentrancy attack. *)
@@ -230,7 +228,7 @@ Definition tokens_to_asset_correct :=
 (* 2 *)
 (* total = 16 *)
 
-(* QuickChick tokens_to_asset_correct. *)
+(* QuickChick (expectFailure tokens_to_asset_correct). *)
 (*
 Begin Trace:
 step_action{Action{act_from: 11%256, act_body: (act_call 130%256, 0, transferhook transfer_descriptor_param{transfer_descr_fa2: 128%256, transfer_descr_batch: [], transfer_descr_operator: 129%256})}}
