execution/tests/EIP20Tests/EIP20TokenGens.v
@@ -77,26 +77,28 @@ Local Close Scope N_scope.
 (* Main generator. *)
 Definition gEIP20TokenAction (env : Environment) : GOpt Action :=
   let call contract_addr caller_addr msg :=
-    returnGenSome {|
-      act_from := caller_addr;
-      act_body := act_call contract_addr 0%Z (serializeMsg msg)
-    |} in
+      returnGenSome {|
+          act_origin := caller_addr;
+          act_from := caller_addr;
+          act_body := act_call contract_addr 0%Z (serializeMsg msg)
+        |} in
   state <- returnGen (get_contract_state EIP20Token.State env contract_addr) ;;
   backtrack [
     (* transfer *)
-    (2, '(caller, msg) <- gTransfer env state ;;
-        call contract_addr caller msg
+      (2, '(caller, msg) <- gTransfer env state ;;
+          call contract_addr caller msg
     ) ;
     (* transfer_from *)
     (3, bindGenOpt (gTransfer_from state)
         (fun '(caller, msg) =>
-        call contract_addr caller msg
+          call contract_addr caller msg
+
         )
     );
     (* approve *)
     (2, bindGenOpt (gApprove state)
         (fun '(caller, msg) =>
-        call contract_addr caller msg
+          call contract_addr caller msg
         )
     )
   ].
